lib/FStar.ListProperties.fst
@@ -320,16 +320,11 @@ let rec sorted f = function
   | [_] -> true
   | x::y::tl -> f x y && sorted f (y::tl)
 
-opaque type total_order (#a:Type) (f: (a -> a -> Tot bool)) =
+type total_order (#a:Type) (f: (a -> a -> Tot bool)) =
     (forall a. f a a)                                           (* reflexivity   *)
     /\ (forall a1 a2. f a1 a2 /\ f a2 a1  ==> a1 = a2)          (* anti-symmetry *)
     /\ (forall a1 a2 a3. f a1 a2 /\ f a2 a3 ==> f a1 a3)        (* transitivity  *)
     /\ (forall a1 a2. f a1 a2 \/ f a2 a1)                       (* totality *)
-
-(* opaque type total_order (a:Type) (f: (a -> a -> Tot bool)) = *)
-(*     (forall a. f a a)                                           (\* reflexivity   *\) *)
-(*     /\ (forall a1 a2. (f a1 a2 /\ a1<>a2)  <==> not (f a2 a1))  (\* anti-symmetry + totality *\) *)
-(*     /\ (forall a1 a2 a3. f a1 a2 /\ f a2 a3 ==> f a1 a3)        (\* transitivity  *\) *)
 
 val append_sorted: #a:Type
                ->  f:(a -> a -> Tot bool)
@@ -341,7 +336,7 @@ val append_sorted: #a:Type
                                     /\ (forall y. mem y l2 ==> f pivot y))
 )                         (ensures (sorted f (l1@(pivot::l2))))
                           [SMTPat (sorted f (l1@(pivot::l2)))]
-let rec append_sorted f l1 l2 pivot = match l1 with
+let rec append_sorted #a f l1 l2 pivot = match l1 with
   | [] -> ()
   | hd::tl -> append_sorted f tl l2 pivot
 
@@ -349,7 +344,7 @@ val sortWithT_sorted: #a:Type -> f:(a -> a -> Tot int) -> l:list a ->
   Lemma (requires (total_order #a (bool_of_compare f)))
         (ensures ((sorted (bool_of_compare f) (sortWithT f l)) /\ (forall x. mem x l = mem x (sortWithT f l))))
         (decreases (length l))
-let rec sortWithT_sorted f l = match l with
+let rec sortWithT_sorted #a f l = match l with
     | [] -> ()
     | pivot::tl ->
        let hi, lo  = partitionT (bool_of_compare f pivot) tl in
